***NO_CI*** wip in decrypt

examples/low-level/crypto/Crypto.AEAD.PRF_MAC.fst
@@ -312,6 +312,23 @@ let prf_mac_wrapper #i #rw aead_st k_0 x =
   in
   mac
 
+val prf_mac_dec
+  (#i:id)
+  (#rw:rw)
+  (aead_st:aead_state i rw)
+  (k_0:CMA.akey aead_st.prf.mac_rgn i)
+  (x:PRF.domain_mac i)
+  : ST (CMA.state (i,x.iv))
+       (requires (fun h0 -> inv aead_st h0))
+       (ensures (fun h0 mac h1 -> prf_mac_ensures i aead_st.prf k_0 x h0 mac h1 /\
+			       inv aead_st h1))
+let prf_mac_dec #i #rw aead_st k_0 x =
+  let h0 = get () in
+  let mac = PRF.prf_mac i aead_st.prf k_0 x in
+  let h1 = get () in
+  frame_inv_prf_mac aead_st k_0 x h0 h1 mac;
+  mac
+
 let post_prf_mac
   (#i:id)
   (#rw:rw)
