examples/low-level/crypto/Crypto.AEAD.Decrypt.fst
@@ -1,0 +1,123 @@
+module Crypto.AEAD.Decrypt
+open FStar.UInt32
+open FStar.Ghost
+open Buffer.Utils
+open FStar.Monotonic.RRef
+
+open Crypto.Indexing
+open Crypto.Symmetric.Bytes
+open Crypto.Plain
+open Flag
+
+open Crypto.Symmetric.PRF
+open Crypto.AEAD.Encoding 
+open Crypto.AEAD.Invariant
+
+module HH       = FStar.HyperHeap
+module HS       = FStar.HyperStack
+module MAC      = Crypto.Symmetric.MAC
+module CMA      = Crypto.Symmetric.UF1CMA
+module Plain    = Crypto.Plain
+module Cipher   = Crypto.Symmetric.Cipher
+module PRF      = Crypto.Symmetric.PRF
+module Dexor       = Crypto.AEAD.EnxorDexor
+module PRF_MAC     = Crypto.AEAD.PRF_MAC
+module Encoding    = Crypto.AEAD.Encoding   
+module EncodingWrapper = Crypto.AEAD.Wrappers.Encoding
+module CMAWrapper = Crypto.AEAD.Wrappers.CMA
+module PRF_MAC    = Crypto.AEAD.PRF_MAC
+
+////////////////////////////////////////////////////////////////////////////////
+//decrypt
+////////////////////////////////////////////////////////////////////////////////
+let decrypt_modifies (#i:id) (#len:u32) (st:aead_state i Reader) (pb:plainBuffer i (v len)) (h0:mem) (h1:mem) =
+   Crypto.AEAD.BufferUtils.decrypt_modifies (safeId i) st.log_region (as_buffer pb) h0 h1
+
+let decrypt_ok (#i:id) (n:Cipher.iv (alg i)) (st:aead_state i Reader) 
+	       (#aadlen:aadlen) (aad:lbuffer (v aadlen))
+	       (#plainlen:txtlen_32)
+	       (plain:plainBuffer i (v plainlen))
+	       (cipher_tagged:lbuffer (v plainlen + v MAC.taglen))
+	       (verified:bool) (h1:mem) = 
+  (enc_dec_liveness st aad plain cipher_tagged h1 /\
+   verified /\ 
+   safeId i) ==> (
+   let aead_entries = HS.sel h1 st.log in 
+   let aad = Buffer.as_seq h1 aad in
+   let plain = Plain.sel_plain h1 plainlen plain in
+   let cipher_tagged = Buffer.as_seq h1 cipher_tagged in 
+   found_matching_entry n aead_entries #aadlen aad plain cipher_tagged)
+
+val decrypt:
+  i:id -> 
+  st:aead_state i Reader ->
+  n:Cipher.iv (alg i) ->
+  aadlen:aadlen ->
+  aad:lbuffer (v aadlen) ->
+  plainlen:txtlen_32 {safelen i (v plainlen) (otp_offset i)} ->
+  plain:plainBuffer i (v plainlen) ->
+  cipher_tagged:lbuffer (v plainlen + v MAC.taglen) ->
+  ST bool
+  (requires (fun h ->
+    enc_dec_separation st aad plain cipher_tagged /\
+    enc_dec_liveness st aad plain cipher_tagged h /\
+    inv st h))
+  (ensures (fun h0 verified h1 ->
+    enc_dec_liveness st aad plain cipher_tagged h1 /\
+    inv st h1 /\
+    decrypt_modifies st plain h0 h1 /\
+    decrypt_ok n st aad plain cipher_tagged verified h1))
+#reset-options "--z3rlimit 1000 --initial_fuel 0 --max_fuel 0 --initial_ifuel 0 --max_ifuel 0"
+let decrypt i st iv aadlen aad plainlen plain cipher_tagged =
+  let h_init = get() in
+  push_frame();
+  let h0 = get () in
+  frame_inv_push st h_init h0;
+  let cipher : lbuffer (v plainlen) = Buffer.sub cipher_tagged 0ul plainlen in
+  let tag = Buffer.sub cipher_tagged plainlen MAC.taglen in
+  let x_0 = PRF.({iv = iv; ctr = ctr_0 i}) in // PRF index to the first block
+  let ak = PRF_MAC.prf_mac_dec st st.ak x_0 in   // used for keying the one-time MAC
+  let h1 = get() in
+(*   assert (prf_mac_modifies i st.prf h0 h1); *)
+  assert(CMA.(MAC.norm h1 ak.r));
+(* // First recompute and check the MAC *)
+  let acc = EncodingWrapper.accumulate ak aad cipher in
+  let h2 = get () in
+  assert (safeId i ==> CMAWrapper.is_mac_for_iv st ak h2);
+  admit()
+  
+  assume (inv st h2);
+  let popt = CMAWrapper.verify st aad plain cipher_tagged ak acc h1 in
+  admit()
+  
+(*   let h2 = ST.get() in *)
+(*   assert (safeId i ==> accumulate_encoded aad #plainlen cipher acc h2); *)
+(*   Buffer.lemma_reveal_modifies_0 h1 h2; *)
+(*   let verified = verify_wrapper ak acc tag in *)
+(*   let h3 = ST.get() in *)
+(*   Buffer.lemma_reveal_modifies_0 h2 h3; *)
+(*   frame_my_inv i st h0 h1 h2 h3; //my_inv st h3 *)
+(*   frame_acc #(i, iv) ak #aadlen aad #plainlen cipher h1 acc h2 h3; *)
+(*   // then, safeID i /\ stateful invariant ==> *)
+(*   //    not verified ==> no entry in the AEAD table *)
+(*   //    verified ==> exists Entry(iv ad l p c) in AEAD.log *)
+(*   //                 and correct entries above x in the PRF table *)
+(*   //                 with matching aad, cipher, and plain *)
+(*   // *)
+(*   // not sure what we need to prove for 1st level of PRF idealization *)
+(*   // possibly that the PRF table with ctr=0 matches the Entry table. *)
+(*   // (PRF[iv,ctr=0].MAC.log =  Some(l,t) iff Entry(iv,___)) *)
+(*   let p = get_verified_plain st aad plain cipher_tagged ak acc verified in  *)
+(*   if verified  *)
+(*   then begin *)
+(*     let y = PRF.incr i x in	    *)
+(*     counter_dexor i st.prf y plainlen plainlen plain cipher p *)
+(*   end; *)
+(*   let h4 = get() in *)
+(*   establish_post_condition st aad plain cipher_tagged p ak acc verified h2 h3 h4; *)
+(*   pop_frame(); *)
+(*   frame_myinv_pop st h4; *)
+(*   frame_decrypt_ok iv st aad plain cipher_tagged verified h4; *)
+(*   chain_modification i iv st aad plain cipher_tagged h_init h0 h1 h2 h3 h4; *)
+(*   verified *)
+
