examples/low-level/crypto/Crypto.AEAD.Wrappers.Encoding.fst
@@ -1,0 +1,103 @@
+module Crypto.AEAD.Wrappers.Encoding 
+
+// This file defines the encoding of additional data and ciphertext
+// authenticated by the one-time MACs, and their injectivity properties. 
+
+open FStar.UInt32
+open FStar.Ghost
+open Buffer.Utils
+open FStar.Monotonic.RRef
+
+open FStar.Math.Lib
+open FStar.Math.Lemmas
+open Crypto.Indexing
+open Crypto.Symmetric.Bytes
+open Crypto.Plain
+open Flag
+
+module HH = FStar.HyperHeap
+module HS = FStar.HyperStack
+
+module MAC = Crypto.Symmetric.MAC
+module CMA = Crypto.Symmetric.UF1CMA
+
+module Cipher   = Crypto.Symmetric.Cipher
+module PRF      = Crypto.Symmetric.PRF
+open Crypto.AEAD.Encoding
+
+////////////////////////////////////////////////////////////////////////////////
+//AEAD.Encoding.accumulate wrapper
+////////////////////////////////////////////////////////////////////////////////
+let accumulate_liveness (#i: MAC.id) (st: CMA.state i) 
+			(#aadlen:aadlen_32) (aad:lbuffer (v aadlen))
+			(#txtlen:txtlen_32) (cipher:lbuffer (v txtlen)) (h:mem) = 
+  MAC.norm h CMA.(st.r) /\
+  Buffer.live h aad /\ 
+  Buffer.live h cipher
+
+// modifies only fresh buffers on the current stack
+let accumulate_modifies_nothing h0 h1 = 
+  let open HS in
+  modifies_one h0.tip h0 h1
+  /\ Buffer.modifies_buf_0 h0.tip h0 h1
+  /\ h0.tip=h1.tip
+
+let fresh_sref (#a:Type0) h0 h1 (r:HS.reference a) = 
+  ~ (h0 `HS.contains` r) /\
+    HS.frameOf r == HS.(h1.tip) /\
+    h1 `HS.contains` r
+
+let accumulate_ensures (#i: MAC.id) (st: CMA.state i) 
+		       (#aadlen:aadlen_32) (aad:lbuffer (v aadlen))
+		       (#txtlen:txtlen_32) (cipher:lbuffer (v txtlen))
+		       (h0:mem) (a:CMA.accBuffer i) (h1:mem) =
+  let open HS in		       
+  let open CMA in 		       
+  accumulate_liveness st aad cipher h1 /\
+  fresh_sref h0 h1 (Buffer.content (MAC.as_buffer a.a)) /\
+  CMA.acc_inv st a h1 /\
+  (mac_log ==> 
+    fresh_sref h0 h1 (alog a) /\
+    HS.sel h1 (alog a) == encode_both (fst i) aadlen (Buffer.as_seq h1 aad) txtlen (Buffer.as_seq h1 cipher))
+
+val frame_accumulate_ensures: #i: MAC.id -> st: CMA.state i -> #aadlen:aadlen_32 -> aad:lbuffer (v aadlen) ->
+	       #txtlen:txtlen_32 -> cipher:lbuffer (v txtlen) -> 
+	       (h0:mem) -> (a:CMA.accBuffer i) -> (h1:mem) -> h2:mem -> 
+    Lemma (requires (accumulate_ensures st aad cipher h0 a h1 /\
+		     Buffer.modifies_0 h1 h2))
+          (ensures (accumulate_ensures st aad cipher h0 a h2))
+#reset-options "--z3rlimit 100 --initial_fuel 0 --max_fuel 0 --initial_ifuel 0 --max_ifuel 0"
+let frame_accumulate_ensures #i st #aalen aad #txtlent cipher h0 a h1 h2 = 
+  FStar.Buffer.lemma_reveal_modifies_0 h1 h2;
+  assert (HS.(h1.tip == h2.tip));
+  assert (h1 `HS.contains` (Buffer.content (MAC.as_buffer CMA.(a.a))));
+  assert (h2 `HS.contains` (Buffer.content (MAC.as_buffer CMA.(a.a))));  
+  assert (fresh_sref h0 h2 (Buffer.content (MAC.as_buffer CMA.(a.a))));
+  if mac_log 
+  then (assert (h1  `HS.contains` CMA.alog a);
+        assert (HS.sel h2 (CMA.alog a) == HS.sel h1 (CMA.alog a));
+	assert (Buffer.as_seq h2 (MAC.as_buffer (CMA.(st.r))) ==
+	        Buffer.as_seq h1 (MAC.as_buffer (CMA.(st.r))));
+        assert (Buffer.as_seq h2 (MAC.as_buffer (CMA.(abuf a))) ==
+                Buffer.as_seq h1 (MAC.as_buffer (CMA.(abuf a))));
+        MAC.frame_sel_elem h1 h2 (CMA.(st.r));
+        MAC.frame_sel_elem h1 h2 (CMA.(abuf a)))
+  else ()
+
+let accumulate (#i: MAC.id) (st: CMA.state i) (#aadlen:aadlen_32) (aad:lbuffer (v aadlen))
+	       (#txtlen:txtlen_32) (cipher:lbuffer (v txtlen))
+   : StackInline (CMA.accBuffer i)
+      (requires (fun h0 -> 
+	  accumulate_liveness st aad cipher h0))
+      (ensures (fun h0 a h1 ->  
+      	  accumulate_liveness st aad cipher h0 /\
+          accumulate_modifies_nothing h0 h1 /\
+	  accumulate_ensures st aad cipher h0 a h1))
+  = let h0 = get () in
+    let acc = accumulate #i st aadlen aad txtlen cipher in
+    let h1 = get () in
+    assert (Buffer.disjoint_2 (MAC.as_buffer (CMA.(acc.a))) (CMA.(st.s)) cipher);
+    assume (mac_log ==> fresh_sref h0 h1 (CMA.alog acc)); //NS: this goes away when Encoding.accumulate is restored
+    assume (fresh_sref h0 h1 (Buffer.content (MAC.as_buffer CMA.(acc.a))));
+    FStar.Buffer.lemma_reveal_modifies_0 h0 h1;
+    acc
